common/Determinism.v
@@ -1,0 +1,508 @@
+(* *********************************************************************)
+(*                                                                     *)
+(*              The Compcert verified compiler                         *)
+(*                                                                     *)
+(*          Xavier Leroy, INRIA Paris-Rocquencourt                     *)
+(*                                                                     *)
+(*  Copyright Institut National de Recherche en Informatique et en     *)
+(*  Automatique.  All rights reserved.  This file is distributed       *)
+(*  under the terms of the INRIA Non-Commercial License Agreement.     *)
+(*                                                                     *)
+(* *********************************************************************)
+
+(** Characterization and properties of deterministic semantics *)
+
+Require Import Classical.
+Require Import Coqlib.
+Require Import AST.
+Require Import Integers.
+Require Import Values.
+Require Import Events.
+Require Import Globalenvs.
+Require Import Smallstep.
+
+(** This file uses classical logic (the axiom of excluded middle), as
+  well as the following extensionality property over infinite
+  sequences of events.  All these axioms are sound in a set-theoretic
+  model of Coq's logic. *)
+
+Axiom traceinf_extensionality:
+  forall T T', traceinf_sim T T' -> T = T'.
+
+(** * Deterministic worlds *)
+
+(** One source of possible nondeterminism is that our semantics leave
+  unspecified the results of calls to external 
+  functions.  Different results to e.g. a "read" operation can of
+  course lead to different behaviors for the program.
+  We address this issue by modeling a notion of deterministic
+  external world that uniquely determines the results of external calls. *)
+
+(** An external world is a function that, given the name of an
+  external call and its arguments, returns either [None], meaning
+  that this external call gets stuck, or [Some(r,w)], meaning
+  that this external call succeeds, has result [r], and changes
+  the world to [w]. *)
+
+Inductive world: Type :=
+  World: (ident -> list eventval -> option (eventval * world)) -> world.
+
+Definition nextworld (w: world) (evname: ident) (evargs: list eventval) :
+                     option (eventval * world) :=
+  match w with World f => f evname evargs end.
+
+(** A trace is possible in a given world if all events correspond
+  to non-stuck external calls according to the given world.
+  Two predicates are defined, for finite and infinite traces respectively:
+- [possible_trace w t w'], where [w] is the initial state of the
+  world, [t] the finite trace of interest, and [w'] the state of the
+  world after performing trace [t].
+- [possible_traceinf w T], where [w] is the initial state of the
+  world and [T] the infinite trace of interest.
+*)
+
+Inductive possible_trace: world -> trace -> world -> Prop :=
+  | possible_trace_nil: forall w,
+      possible_trace w E0 w
+  | possible_trace_cons: forall w0 evname evargs evres w1 t w2,
+      nextworld w0 evname evargs = Some (evres, w1) ->
+      possible_trace w1 t w2 ->
+      possible_trace w0 (mkevent evname evargs evres :: t) w2.
+
+Lemma possible_trace_app:
+  forall t2 w2 w0 t1 w1,
+  possible_trace w0 t1 w1 -> possible_trace w1 t2 w2 ->
+  possible_trace w0 (t1 ** t2) w2.
+Proof.
+  induction 1; simpl; intros.
+  auto.
+  econstructor; eauto.
+Qed.
+
+Lemma possible_trace_app_inv:
+  forall t2 w2 t1 w0,
+  possible_trace w0 (t1 ** t2) w2 ->
+  exists w1, possible_trace w0 t1 w1 /\ possible_trace w1 t2 w2.
+Proof.
+  induction t1; simpl; intros.
+  exists w0; split. constructor. auto.
+  inv H. exploit IHt1; eauto. intros [w1 [A B]]. 
+  exists w1; split. econstructor; eauto. auto.
+Qed.
+
+CoInductive possible_traceinf: world -> traceinf -> Prop :=
+  | possible_traceinf_cons: forall w0 evname evargs evres w1 T,
+      nextworld w0 evname evargs = Some (evres, w1) ->
+      possible_traceinf w1 T ->
+      possible_traceinf w0 (Econsinf (mkevent evname evargs evres) T).
+
+Lemma possible_traceinf_app:
+  forall t2 w0 t1 w1,
+  possible_trace w0 t1 w1 -> possible_traceinf w1 t2 ->
+  possible_traceinf w0 (t1 *** t2).
+Proof.
+  induction 1; simpl; intros.
+  auto.
+  econstructor; eauto.
+Qed.
+
+Lemma possible_traceinf_app_inv:
+  forall t2 t1 w0,
+  possible_traceinf w0 (t1 *** t2) ->
+  exists w1, possible_trace w0 t1 w1 /\ possible_traceinf w1 t2.
+Proof.
+  induction t1; simpl; intros.
+  exists w0; split. constructor. auto.
+  inv H. exploit IHt1; eauto. intros [w1 [A B]]. 
+  exists w1; split. econstructor; eauto. auto.
+Qed.
+
+Ltac possibleTraceInv :=
+  match goal with
+  | [H: possible_trace _ E0 _ |- _] =>
+      inversion H; clear H; subst; possibleTraceInv
+  | [H: possible_trace _ (_ ** _) _ |- _] =>
+      let P1 := fresh "P" in
+      let w := fresh "w" in
+      let P2 := fresh "P" in
+      elim (possible_trace_app_inv _ _ _ _ H); clear H;
+      intros w [P1 P2];
+      possibleTraceInv
+  | [H: possible_traceinf _ (_ *** _) |- _] =>
+      let P1 := fresh "P" in
+      let w := fresh "w" in
+      let P2 := fresh "P" in
+      elim (possible_traceinf_app_inv _ _ _ H); clear H;
+      intros w [P1 P2];
+      possibleTraceInv
+  | [H: exists w, possible_trace _ _ w |- _] =>
+      let P := fresh "P" in let w := fresh "w" in 
+      destruct H as [w P]; possibleTraceInv
+  | _ => idtac
+  end.
+
+Definition possible_behavior (w: world) (b: program_behavior) : Prop :=
+  match b with
+  | Terminates t r => exists w', possible_trace w t w'
+  | Diverges t => exists w', possible_trace w t w'
+  | Reacts T => possible_traceinf w T
+  | Goes_wrong t => exists w', possible_trace w t w'
+  end.
+
+(** Determinism properties of [event_match]. *)
+
+Remark eventval_match_deterministic:
+  forall ev1 ev2 ty v1 v2,
+  eventval_match ev1 ty v1 -> eventval_match ev2 ty v2 ->
+  (ev1 = ev2 <-> v1 = v2).
+Proof.
+  intros. inv H; inv H0; intuition congruence.
+Qed.
+
+Remark eventval_list_match_deterministic:
+  forall ev1 ty v, eventval_list_match ev1 ty v ->
+  forall ev2, eventval_list_match ev2 ty v -> ev1 = ev2.
+Proof.
+  induction 1; intros.
+  inv H. auto.
+  inv H1. decEq.
+  rewrite (eventval_match_deterministic _ _ _ _ _ H H6). auto.
+  eauto.
+Qed.
+
+(** * Deterministic semantics *)
+
+Section DETERM_SEM.
+
+(** We assume given a transition semantics that is internally
+  deterministic: the only source of non-determinism is the return
+  value of external calls. *)
+
+Variable genv: Type.
+Variable state: Type.
+Variable step: genv -> state -> trace -> state -> Prop.
+Variable initial_state: state -> Prop.
+Variable final_state: state -> int -> Prop.
+
+Inductive internal_determinism: trace -> state -> trace -> state -> Prop :=
+  | int_determ_0: forall s,
+      internal_determinism E0 s E0 s
+  | int_determ_1: forall s s' id arg res res',
+      (res = res' -> s = s') ->
+      internal_determinism (mkevent id arg res :: nil) s
+                           (mkevent id arg res' :: nil) s'.
+
+Hypothesis step_internal_deterministic:
+  forall ge s t1 s1 t2 s2,
+  step ge s t1 s1 -> step ge s t2 s2 -> internal_determinism t1 s1 t2 s2.
+
+Hypothesis initial_state_determ:
+  forall s1 s2, initial_state s1 -> initial_state s2 -> s1 = s2.
+
+Hypothesis final_state_determ:
+  forall st r1 r2, final_state st r1 -> final_state st r2 -> r1 = r2.
+
+Hypothesis final_state_nostep:
+  forall ge st r, final_state st r -> nostep step ge st.
+
+(** Consequently, the [step] relation is deterministic if restricted
+    to traces that are possible in a deterministic world. *)
+
+Lemma step_deterministic:
+  forall ge s0 t1 s1 t2 s2 w0 w1 w2,
+  step ge s0 t1 s1 -> step ge s0 t2 s2 ->
+  possible_trace w0 t1 w1 -> possible_trace w0 t2 w2 ->
+  s1 = s2 /\ t1 = t2 /\ w1 = w2.
+Proof.
+  intros. exploit step_internal_deterministic. eexact H. eexact H0. intro ID.
+  inv ID.
+  inv H1. inv H2. auto.
+  inv H2. inv H11. inv H1. inv H11. 
+  rewrite H10 in H9. inv H9. 
+  intuition.
+Qed.
+
+Ltac use_step_deterministic :=
+  match goal with
+  | [ S1: step _ _ ?t1 _, P1: possible_trace _ ?t1 _,
+      S2: step _ _ ?t2 _, P2: possible_trace _ ?t2 _ |- _ ] =>
+    destruct (step_deterministic _ _ _ _ _ _ _ _ _ S1 S2 P1 P2)
+    as [EQ1 [EQ2 EQ3]]; subst
+  end.
+
+(** Determinism for finite transition sequences. *)
+
+Lemma star_step_diamond:
+  forall ge s0 t1 s1, star step ge s0 t1 s1 -> 
+  forall t2 s2 w0 w1 w2, star step ge s0 t2 s2 -> 
+  possible_trace w0 t1 w1 -> possible_trace w0 t2 w2 ->
+  exists t,
+     (star step ge s1 t s2 /\ possible_trace w1 t w2 /\ t2 = t1 ** t)
+  \/ (star step ge s2 t s1 /\ possible_trace w2 t w1 /\ t1 = t2 ** t).
+Proof.
+  induction 1; intros. 
+  inv H0. exists t2; auto. 
+  inv H2. inv H4. exists (t1 ** t2); right. 
+    split. econstructor; eauto. auto.
+  possibleTraceInv. use_step_deterministic.  
+  exploit IHstar. eexact H6. eauto. eauto. 
+  intros [t A]. exists t.
+  destruct A. left; intuition. traceEq. right; intuition. traceEq. 
+Qed.
+
+Ltac use_star_step_diamond :=
+  match goal with
+  | [ S1: star step _ _ ?t1 _, P1: possible_trace _ ?t1 _,
+      S2: star step _ _ ?t2 _, P2: possible_trace _ ?t2 _ |- _ ] =>
+    let t := fresh "t" in let P := fresh "P" in let Q := fresh "Q" in let EQ := fresh "EQ" in
+    destruct (star_step_diamond _ _ _ _ S1 _ _ _ _ _ S2 P1 P2)
+    as [t [ [P [Q EQ]] | [P [Q EQ]] ]]; subst
+  end.
+
+Ltac use_nostep :=
+  match goal with
+  | [ S: step _ ?s _ _, NO: nostep step _ ?s |- _ ] => elim (NO _ _ S)
+  end.
+
+Lemma star_step_triangle:
+  forall ge s0 t1 s1 t2 s2 w0 w1 w2,
+  star step ge s0 t1 s1 -> 
+  star step ge s0 t2 s2 -> 
+  possible_trace w0 t1 w1 -> possible_trace w0 t2 w2 ->
+  nostep step ge s2 ->
+  exists t,
+  star step ge s1 t s2 /\ possible_trace w1 t w2 /\ t2 = t1 ** t.
+Proof.
+  intros. use_star_step_diamond; possibleTraceInv. 
+  exists t; auto.
+  inv P. inv Q. exists E0. split. constructor. split. constructor. traceEq.
+  use_nostep.
+Qed.
+
+Ltac use_star_step_triangle :=
+  match goal with
+  | [ S1: star step _ _ ?t1 _, P1: possible_trace _ ?t1 _,
+      S2: star step _ _ ?t2 ?s2, P2: possible_trace _ ?t2 _,
+      NO: nostep step _ ?s2 |- _ ] =>
+    let t := fresh "t" in let P := fresh "P" in let Q := fresh "Q" in let EQ := fresh "EQ" in
+    destruct (star_step_triangle _ _ _ _ _ _ _ _ _ S1 S2 P1 P2 NO)
+    as [t [P [Q EQ]]]; subst
+  end.
+
+Lemma steps_deterministic:
+  forall ge s0 t1 s1 t2 s2 w0 w1 w2,
+  star step ge s0 t1 s1 -> star step ge s0 t2 s2 -> 
+  nostep step ge s1 -> nostep step ge s2 ->
+  possible_trace w0 t1 w1 -> possible_trace w0 t2 w2 ->
+  t1 = t2 /\ s1 = s2.
+Proof.
+  intros. use_star_step_triangle. inv P.
+  inv Q. split; auto; traceEq. use_nostep.
+Qed.
+
+Lemma terminates_not_goes_wrong:
+  forall ge s t1 s1 r w w1 t2 s2 w2,
+  star step ge s t1 s1 -> final_state s1 r -> possible_trace w t1 w1 ->
+  star step ge s t2 s2 -> nostep step ge s2 -> possible_trace w t2 w2 ->
+  (forall r, ~final_state s2 r) -> False.
+Proof.
+  intros.
+  assert (t1 = t2 /\ s1 = s2). 
+    eapply steps_deterministic; eauto. 
+  destruct H6; subst. elim (H5 _ H0).
+Qed.
+
+(** Determinism for infinite transition sequences. *)
+
+Lemma star_final_not_forever_silent:
+  forall ge s t s', star step ge s t s' ->
+  forall w w', possible_trace w t w' -> nostep step ge s' ->
+  forever_silent step ge s -> False.
+Proof.
+  induction 1; intros. 
+  inv H1. use_nostep. 
+  inv H4. possibleTraceInv. assert (possible_trace w E0 w) by constructor. 
+  use_step_deterministic. eauto.
+Qed.
+
+Lemma star2_final_not_forever_silent:
+  forall ge s t1 s1 w w1 t2 s2 w2,
+  star step ge s t1 s1 -> possible_trace w t1 w1 -> nostep step ge s1 ->
+  star step ge s t2 s2 -> possible_trace w t2 w2 -> forever_silent step ge s2 ->
+  False.
+Proof.
+  intros. use_star_step_triangle. possibleTraceInv. 
+  eapply star_final_not_forever_silent. eexact P. eauto. auto. auto.
+Qed.
+
+Lemma star_final_not_forever_reactive:
+  forall ge s t s', star step ge s t s' -> 
+  forall w w' T, possible_trace w t w' -> possible_traceinf w T -> nostep step ge s' ->
+  forever_reactive step ge s T -> False.
+Proof.
+  induction 1; intros.
+  inv H2. inv H3. congruence. use_nostep. 
+  inv H5. possibleTraceInv. inv H6. congruence. possibleTraceInv.
+  use_step_deterministic.
+  eapply IHstar with (T := t4 *** T0). eauto. 
+  eapply possible_traceinf_app; eauto. auto. 
+  eapply star_forever_reactive; eauto.  
+Qed.
+
+Lemma star_forever_silent_inv:
+  forall ge s t s', star step ge s t s' ->
+  forall w w', possible_trace w t w' ->
+  forever_silent step ge s -> 
+  t = E0 /\ forever_silent step ge s'.
+Proof.
+  induction 1; intros.
+  auto.
+  subst. possibleTraceInv. inv H3. assert (possible_trace w E0 w) by constructor.
+  use_step_deterministic. eauto. 
+Qed.
+
+Lemma forever_silent_reactive_exclusive:
+  forall ge s w T,
+  forever_silent step ge s -> forever_reactive step ge s T -> 
+  possible_traceinf w T -> False.
+Proof.
+  intros. inv H0. possibleTraceInv. exploit star_forever_silent_inv; eauto. 
+  intros [A B]. contradiction.
+Qed.
+
+Lemma forever_reactive_inv2:
+  forall ge s t1 s1, star step ge s t1 s1 ->
+  forall t2 s2 T1 T2 w w1 w2,
+  possible_trace w t1 w1 ->
+  star step ge s t2 s2 -> possible_trace w t2 w2 ->
+  t1 <> E0 -> t2 <> E0 ->
+  forever_reactive step ge s1 T1 -> possible_traceinf w1 T1 ->
+  forever_reactive step ge s2 T2 -> possible_traceinf w2 T2 ->
+  exists s', exists e, exists T1', exists T2', exists w',
+  forever_reactive step ge s' T1' /\ possible_traceinf w' T1' /\
+  forever_reactive step ge s' T2' /\ possible_traceinf w' T2' /\
+  t1 *** T1 = Econsinf e T1' /\
+  t2 *** T2 = Econsinf e T2'.
+Proof.
+  induction 1; intros.
+  congruence.
+  inv H3. congruence. possibleTraceInv.
+  assert (ID: internal_determinism t3 s5 t1 s2). eauto. 
+  inv ID.
+  possibleTraceInv. eauto.
+  inv P. inv P1. inv H17. inv H19. rewrite H18 in H16; inv H16.
+  assert (s5 = s2) by auto. subst s5.
+  exists s2; exists (mkevent id arg res');
+  exists (t2 *** T1); exists (t4 *** T2); exists w0.
+  split. eapply star_forever_reactive; eauto. 
+  split. eapply possible_traceinf_app; eauto. 
+  split. eapply star_forever_reactive; eauto. 
+  split. eapply possible_traceinf_app; eauto.
+  auto.
+Qed.
+
+Lemma forever_reactive_determ:
+  forall ge s T1 T2 w,
+  forever_reactive step ge s T1 -> possible_traceinf w T1 ->
+  forever_reactive step ge s T2 -> possible_traceinf w T2 ->
+  traceinf_sim T1 T2.
+Proof.
+  cofix COINDHYP; intros.
+  inv H. inv H1. possibleTraceInv.
+  destruct (forever_reactive_inv2 _ _ _ _ H _ _ _ _ _ _ _ P H3 P1 H6 H4
+                                  H7 P0 H5 P2)
+  as [s' [e [T1' [T2' [w' [A [B [C [D [E G]]]]]]]]]].
+  rewrite E; rewrite G. constructor.
+  eapply COINDHYP; eauto. 
+Qed.
+
+Lemma star_forever_reactive_inv:
+  forall ge s t s', star step ge s t s' ->
+  forall w w' T, possible_trace w t w' -> forever_reactive step ge s T ->
+  possible_traceinf w T ->
+  exists T', forever_reactive step ge s' T' /\ possible_traceinf w' T' /\ T = t *** T'.
+Proof.
+  induction 1; intros. 
+  possibleTraceInv. exists T; auto.
+  inv H3. possibleTraceInv. inv H5. congruence. possibleTraceInv.
+  use_step_deterministic. 
+  exploit IHstar. eauto. eapply star_forever_reactive. 2: eauto. eauto.
+  eapply possible_traceinf_app; eauto. 
+  intros [T' [A [B C]]]. exists T'; intuition. traceEq. congruence. 
+Qed.
+
+Lemma forever_silent_reactive_exclusive2:
+  forall ge s t s' w w' T,
+  star step ge s t s' -> possible_trace w t w' -> forever_silent step ge s' ->
+  forever_reactive step ge s T -> possible_traceinf w T ->
+  False.
+Proof.
+  intros. exploit star_forever_reactive_inv; eauto. 
+  intros [T' [A [B C]]]. subst T.
+  eapply forever_silent_reactive_exclusive; eauto.
+Qed.
+
+(** Determinism for program executions *)
+
+Ltac use_init_state :=
+  match goal with
+  | [ H1: (initial_state _), H2: (initial_state _) |- _ ] =>
+        generalize (initial_state_determ _ _ H1 H2); intro; subst; clear H2
+  | [ H1: (initial_state _), H2: (forall s, ~initial_state s) |- _ ] =>
+        elim (H2 _ H1)
+  | _ => idtac
+  end.
+
+Theorem program_behaves_deterministic:
+  forall ge w beh1 beh2,
+  program_behaves step initial_state final_state ge beh1 -> possible_behavior w beh1 ->
+  program_behaves step initial_state final_state ge beh2 -> possible_behavior w beh2 ->
+  beh1 = beh2.
+Proof.
+  intros until beh2; intros BEH1 POS1 BEH2 POS2.
+  inv BEH1; inv BEH2; simpl in POS1; simpl in POS2;
+  possibleTraceInv; use_init_state.
+(* terminates, terminates *)
+  assert (t = t0 /\ s' = s'0). eapply steps_deterministic; eauto.
+  destruct H2. f_equal; auto. subst. eauto. 
+(* terminates, diverges *)
+  byContradiction. eapply star2_final_not_forever_silent with (s1 := s') (s2 := s'0); eauto.
+(* terminates, reacts *)
+  byContradiction. eapply star_final_not_forever_reactive; eauto.
+(* terminates, goes_wrong *)
+  byContradiction. eapply terminates_not_goes_wrong with (s1 := s') (s2 := s'0); eauto.
+(* diverges, terminates *)
+  byContradiction. eapply star2_final_not_forever_silent with (s2 := s') (s1 := s'0); eauto.
+(* diverges, diverges *)
+  f_equal. use_star_step_diamond.
+  exploit star_forever_silent_inv. eexact P1. eauto. eauto.
+  intros [A B]. subst; traceEq.
+  exploit star_forever_silent_inv. eexact P1. eauto. eauto.
+  intros [A B]. subst; traceEq.
+(* diverges, reacts *)
+  byContradiction. eapply forever_silent_reactive_exclusive2; eauto.
+(* diverges, goes wrong *)
+  byContradiction. eapply star2_final_not_forever_silent with (s1 := s'0) (s2 := s'); eauto.
+(* reacts, terminates *)
+  byContradiction. eapply star_final_not_forever_reactive; eauto.
+(* reacts, diverges *) 
+  byContradiction. eapply forever_silent_reactive_exclusive2; eauto.
+(* reacts, reacts *)
+  f_equal. apply traceinf_extensionality. 
+  eapply forever_reactive_determ; eauto. 
+(* reacts, goes wrong *)
+  byContradiction. eapply star_final_not_forever_reactive; eauto.
+(* goes wrong, terminate *)
+  byContradiction. eapply terminates_not_goes_wrong with (s1 := s'0) (s2 := s'); eauto.
+(* goes wrong, diverges *)
+  byContradiction. eapply star2_final_not_forever_silent with (s1 := s') (s2 := s'0); eauto.
+(* goes wrong, reacts *)
+  byContradiction. eapply star_final_not_forever_reactive; eauto.
+(* goes wrong, goes wrong *)
+  assert (t = t0 /\ s' = s'0). eapply steps_deterministic; eauto.
+  destruct H3. congruence.
+(* goes initially wrong, goes initially wrong *)
+  reflexivity.
+Qed.
+
+End DETERM_SEM.
